Stronger AG iterW lemma and prove ghost property for Sec.v

examples/Sec.v
@@ -63,9 +63,10 @@ Proof.
 Qed.
 
 Lemma sec_lte_H(l: Sec): l ⪯ H.
-Proof.
-  destruct l; repeat econstructor.
-Qed.
+Proof. destruct l; repeat econstructor. Qed.
+
+Lemma sec_lte_L(l: Sec): L ⪯ l.
+Proof. destruct l; repeat econstructor. Qed.
 
 (*| Both values and addresses are nat |*)
 Notation Addr := nat.
@@ -82,16 +83,26 @@ Section SecurityEx.
           | Read l addr => option nat
           | Write l addr v => unit
           end.
-
+  
+  (* Ghost state, instrument every read with
+     [m: memory address it targets]
+     [ml: Security-level of the instruction]
+     [al: Security-level of the address cell previously written]
+   *)               
+  Record SecObs := { ml: Sec; al: Sec }.
+  
   (* Insecure interpreter, does not check labels *)
-  Definition h_secE: secE ~> stateT St (ctree void) :=
+  Definition h_secE: secE ~> stateT St (ctreeW SecObs) :=
     fun e => mkStateT
             (fun (st: St) =>                                     
-               match e return ctree void (encode e * St) with
-               | Read _ addr =>                                 
+               match e return ctreeW SecObs (encode e * St) with
+               | Read l addr =>
                    match lookup addr st with
                    (* [addr] exists and set to [(v, l_a)] *)
-                   | Some (l_a, v) => Ret (Some v, st)
+                   | Some (l_a, v) =>
+                       (* Instrumentation *)
+                       log {| ml:=l_a; al := l |} ;;
+                       Ret (Some v, st)
                    (* [addr] does not exist, return [None] *)
                    | None => Ret (None, st)
                    end
@@ -100,16 +111,6 @@ Section SecurityEx.
                    Ret (tt, add addr (l, v) st)
                end).
 
-  (* Ghost state, instrument every read with
-     [m: memory address it targets]
-     [ml: Security-level of the instruction]
-     [al: Security-level of the address cell previously written]
-   *)
-               
-  (* Instrumented semantics, simply log every successful read with [readG] *)
-  Definition h_secE_instr: secE ~> stateT St (ctreeW St) :=
-    h_writerΣ h_secE.
-  
   (* Trigger instructions *)
   Definition read: Sec -> Addr -> ctree secE (option nat) :=
     fun (l: Sec) (addr: Addr) => Ctree.trigger (Read l addr). 
@@ -144,24 +145,23 @@ Section SecurityEx.
             (sec_bob1 i));;
          (* Increase counter by 1 *)
          Ret (S i)) 0.
-  
-  Definition noleak(i: Addr) (σ: St) : Prop :=
-    Nat.Even i ->
-    exists v, lookup i σ = Some (L, v).
+
+  Definition no_leak(i: Addr) (σ: St): Prop :=
+    Nat.Even i -> exists v, lookup i σ = Some (L, v).
 
   (* Safety property: there does not exist a memory label [ml] accessed by
      label [al ≺ ml], or there does not exist a low intruction that reads from
      high-security memory *)
   Typeclasses Transparent equ.
   Theorem ag_safety_sec: forall (secret: nat) (σ: St),
-      (forall i, noleak i σ) ->
-      <( {interp_state h_secE_instr (sec_system secret) σ},
-         {Obs (Log σ) tt} |= AG visW {fun σ => forall i, noleak i σ} )>.
+      (forall i, no_leak i σ) ->
+      <( {interp_state h_secE (sec_system secret) σ},
+         {Obs (Log {| ml := L; al := L |}) tt} |= AG visW {fun obs => obs.(al) ⪯ obs.(ml)} )>.
   Proof with eauto with ctl.
     intros.    
     unfold sec_system, forever.
-    apply ag_iterW with (R:=fun _ => True)...
-    intros i σ' [] Hσ0. 
+    apply ag_iterW with (R:=fun _ σ => forall i, no_leak i σ)...
+    intros i σ' [] Hσ0 Hφ; cbn in Hφ.
     rewrite map_bind, interp_state_bind.
     unfold br2.
     rewrite interp_state_br.
@@ -178,15 +178,8 @@ Section SecurityEx.
     - (* Alice runs, [i] is even *)
       eapply au_bind_r_eq.
       + rewrite (@interp_state_trigger _ _ _ _ _ _ (Write H (S i) secret) _); cbn.
-        rewrite bind_bind, resumCtree_ret', bind_ret_l.
-        eapply au_bind_r_eq; [eapply au_bind_r_eq|].
-        * apply au_vis_l...
-           -- apply ctl_vis...
-           -- intros [].
-              cright; apply ax_done...
-        * cright; apply ax_done...
-        * apply au_guard.
-          cright; apply ax_done...
+        rewrite bind_ret_l, sb_guard.
+        cright; apply ax_done...
       + cbn.
         rewrite interp_state_ret.
         cright; apply ax_done; split...
@@ -194,121 +187,93 @@ Section SecurityEx.
         do 2 eexists; split...
         cbn; intuition.
         eexists; intuition.
-        * intro Heven.
-          unfold noleak in *.
-          destruct (Nat.eq_dec i0 (S i)).
-          -- (* i0 = S i *)
-            rewrite e0 in Heven.
-            apply Nat.Even_succ in Heven.
-            exfalso.
-            apply Nat.Even_Odd_False with i...
-          -- (* i0 <> S i *)
-            destruct (Hσ0 i0 Heven) as (v & ?).
-            exists v.
-            rewrite OF.(mapsto_lookup).
-            apply mapsto_add_neq with (R:=eq); auto.
-            now rewrite <- mapsto_lookup.
+        intro Heven.
+        destruct (Hσ0 i0 Heven) as (v & ?); exists v.
+        destruct (Nat.eq_dec i0 (S i)).
+        * (* i0 = S i *)
+          rewrite e0 in Heven.
+          exfalso.
+          apply Nat.Even_succ in Heven.
+          apply Nat.Even_Odd_False with i...
+        * (* i0 <> i *)
+          rewrite OF.(mapsto_lookup).
+          apply mapsto_add_neq with (R:=eq); auto.
+          now rewrite <- mapsto_lookup.
     - (* Alice runs, [i] is odd *)
       eapply au_bind_r_eq.
       + rewrite (@interp_state_trigger _ _ _ _ _ _ (Write H i secret) _); cbn.
-        rewrite bind_bind, resumCtree_ret', bind_ret_l.
+        rewrite bind_ret_l, sb_guard.
+        cright; apply ax_done...
+      + cbn.
+        rewrite interp_state_ret.
+        cright; apply ax_done; split...
+        eexists; split...
+        do 2 eexists; split...
+        cbn; intuition.
+        eexists; intuition.
+        intro Heven.
+        destruct (Hσ0 i0 Heven) as (v & ?); exists v.
+        destruct (Nat.eq_dec i0 i).
+        * (* i0 = i *)
+          rewrite e in Heven.
+          exfalso.
+          apply Nat.Even_Odd_False with i...
+        * (* i0 <> i *)
+          rewrite OF.(mapsto_lookup).
+          apply mapsto_add_neq with (R:=eq); auto.
+          now rewrite <- mapsto_lookup.
+    - (* Bob runs, [i] is even *)
+      rewrite interp_state_bind, bind_bind.
+      rewrite (@interp_state_trigger _ _ _ _ _ _ (Read L i) _); cbn.
+      rewrite bind_bind.
+      destruct (lookup i σ') eqn:Hlook.
+      + destruct p as (l, a).
         eapply au_bind_r_eq; [eapply au_bind_r_eq|].
         * apply au_vis_l...
           -- apply ctl_vis...
           -- intros [].
              cright; apply ax_done...
         * cright; apply ax_done...
-        * cbn.
-          apply au_guard.
-          cright; apply ax_done...
-      + cbn.
-        rewrite interp_state_ret.
-        cright; apply ax_done; split...
-        eexists; split...
-        do 2 eexists; split...
-        cbn; intuition.
+        * rewrite bind_guard, sb_guard, bind_ret_l, interp_state_ret, bind_ret_l,
+            interp_state_ret.
+          cright; apply ax_done; split...
+          eexists; intuition.
+          do 2 eexists; intuition.
+          cbn.
+          eexists; intuition.
+          apply sec_lte_L.
+      + rewrite bind_ret_l, bind_guard, sb_guard, bind_ret_l, interp_state_ret,
+          bind_ret_l, interp_state_ret.
+        cright; apply ax_done; intuition...
         eexists; intuition.
-        * intro Heven.
-          unfold noleak in *.
-          destruct (Nat.eq_dec i0 i).
-          -- (* i0 = i *)
-            rewrite e in Heven.
-            exfalso.
-            apply Nat.Even_Odd_False with i...
-          -- (* i0 <> i *)
-            destruct (Hσ0 i0 Heven) as (v & ?).
-            exists v.
-            rewrite OF.(mapsto_lookup).
-            apply mapsto_add_neq with (R:=eq); auto.
-            now rewrite <- mapsto_lookup.
-    - (* Bob runs, [i] is even *)
-      eapply au_bind_r_eq.
-      + rewrite interp_state_bind.
-        rewrite (@interp_state_trigger _ _ _ _ _ _ (Read L i) _); cbn.
-        rewrite ?bind_bind.          
-        destruct (lookup i σ') eqn:Hlook.
-        * destruct p as (l, a).
-          rewrite resumCtree_ret', bind_ret_l, bind_bind.
-          -- eapply au_bind_r_eq; [eapply au_bind_r_eq|].
-             ++ apply au_vis_l...
-                ** apply ctl_vis...
-                ** intros [].
-                   cright; apply ax_done...
-             ++ rewrite bind_ret_l, sb_guard.
-                cright; apply ax_done...
-             ++ cbn.
-                rewrite interp_state_ret.
-                cright; apply ax_done...
-        * rewrite resumCtree_ret', bind_ret_l, ?bind_bind.
-          eapply au_bind_r_eq. 
-          -- apply au_vis_l...
-             apply ctl_vis...
-             intros [].
-             cright; apply ax_done...
-          -- rewrite bind_bind, bind_ret_l, bind_guard, sb_guard, bind_ret_l,
-               interp_state_ret.
-             cright; apply ax_done...
-      + cbn.
-        rewrite interp_state_ret.
-        cright; apply ax_done; split...
-        eexists; split...
-        do 2 eexists; split...
-        cbn; intuition.
+        do 2 eexists; intuition.
         eexists; intuition.
     - (* Bob runs, [i] is odd *)
-      eapply au_bind_r_eq.
-      + rewrite interp_state_bind.
-        rewrite (@interp_state_trigger _ _ _ _ _ _ (Read L (S i)) _); cbn.
-        repeat rewrite bind_bind.          
-        destruct (lookup (S i) σ') eqn:Hlook.
-        * destruct p as (l, a).
-          rewrite resumCtree_ret', bind_ret_l, bind_bind.
-          -- eapply au_bind_r_eq; [eapply au_bind_r_eq|].
-             ++ apply au_vis_l...
-                ** apply ctl_vis...
-                ** intros [].
-                   cright; apply ax_done...
-             ++ rewrite bind_ret_l, sb_guard.
-                cright; apply ax_done...
-             ++ cbn.
-                rewrite interp_state_ret.
-                cright; apply ax_done...
-        * rewrite resumCtree_ret', bind_ret_l, ?bind_bind.
-          eapply au_bind_r_eq. 
-          -- apply au_vis_l...
-             apply ctl_vis...
-             intros [].
+      rewrite interp_state_bind, bind_bind.
+      rewrite (@interp_state_trigger _ _ _ _ _ _ (Read L (S i)) _); cbn.
+      rewrite bind_bind.
+      destruct (lookup (S i) σ') eqn:Hlook.
+      + destruct p as (l, a).
+        eapply au_bind_r_eq; [eapply au_bind_r_eq|].
+        * apply au_vis_l...
+          -- apply ctl_vis...
+          -- intros [].
              cright; apply ax_done...
-          -- rewrite bind_bind, bind_ret_l, bind_guard, sb_guard, bind_ret_l,
-               interp_state_ret.
-             cright; apply ax_done...
-      + cbn.
-        rewrite interp_state_ret.
-        cright; apply ax_done; split...
-        eexists; split...
-        do 2 eexists; split...
-        cbn; intuition.
+        * cright; apply ax_done...
+        * rewrite bind_guard, sb_guard, bind_ret_l, interp_state_ret, bind_ret_l,
+            interp_state_ret.
+          cright; apply ax_done; split...
+          eexists; intuition.
+          do 2 eexists; intuition.
+          cbn.
+          eexists; intuition.
+          apply sec_lte_L.
+      + rewrite bind_ret_l, bind_guard, sb_guard, bind_ret_l, interp_state_ret,
+          bind_ret_l, interp_state_ret.
+        cright; apply ax_done; intuition...
         eexists; intuition.
-  Qed.
+        do 2 eexists; intuition.
+        eexists; intuition.
+  Qed.        
   Print Assumptions ag_safety_sec.
 End SecurityEx.
